theories/core/utp_assert.thy
@@ -1,0 +1,49 @@
+(******************************************************************************)
+(* Project: Unifying Theories of Programming in HOL                           *)
+(* File: utp_assert.thy                                                       *)
+(* Author: Simon Foster, University of York (UK)                              *)
+(******************************************************************************)
+
+header {* Assertions and Assumptions *}
+
+theory utp_assert
+imports 
+  utp_lattice
+begin
+
+definition AssertR ::
+"'VALUE WF_PREDICATE \<Rightarrow>
+ 'VALUE WF_PREDICATE" ("_\<^sub>\<bottom>" [200] 200) where
+"c\<^sub>\<bottom> \<equiv> II \<lhd> c \<rhd> \<bottom>"
+
+definition AssumeR ::
+"'VALUE WF_PREDICATE \<Rightarrow>
+ 'VALUE WF_PREDICATE" ("_\<^sup>\<top>" [200] 200) where
+"c\<^sup>\<top> \<equiv> II \<lhd> c \<rhd> \<top>"
+
+syntax
+  "_upred_assert" :: "upred \<Rightarrow> upred" ("_\<^sub>\<bottom>" [900] 900)
+  "_upred_assume" :: "upred \<Rightarrow> upred" ("_\<^sup>\<top>" [899] 899)
+
+translations
+  "_upred_assert c" == "CONST AssertR c"
+  "_upred_assume c" == "CONST AssumeR c"
+
+lemma UNREST_AssumeR_DASHED_TWICE [unrest]:
+  "UNREST DASHED_TWICE c \<Longrightarrow> UNREST DASHED_TWICE (c\<^sup>\<top>)"
+  by (force intro:unrest simp add: AssumeR_def)
+
+lemma UNREST_AssertR_DASHED_TWICE [unrest]:
+  "UNREST DASHED_TWICE c \<Longrightarrow> UNREST DASHED_TWICE (c\<^sub>\<bottom>)"
+  by (force intro:unrest simp add: AssertR_def)
+
+declare AssumeR_def [eval, evalr, evalrr, evalrx]
+declare AssertR_def [eval, evalr, evalrr, evalrx]
+
+lemma AssertR_SemiR:
+  "\<lbrakk> b \<in> WF_CONDITION; c \<in> WF_CONDITION \<rbrakk> \<Longrightarrow> b\<^sub>\<bottom> ; c\<^sub>\<bottom> = (b \<and>\<^sub>p c)\<^sub>\<bottom>"
+  apply (frule SemiR_TrueP_precond, frule SemiR_TrueP_precond) back
+  apply (utp_xrel_auto_tac)
+done
+
+end
