theories/core/utp_core.thy
@@ -16,7 +16,9 @@ imports
   utp_pred
   utp_rename
   utp_lattice
+  utp_assert
   utp_recursion
+  utp_iteration
   utp_unrest
   utp_rel
   utp_wp
