theories/core/utp_iteration.thy
@@ -1,0 +1,205 @@
+(******************************************************************************)
+(* Project: Unifying Theories of Programming in HOL                           *)
+(* File: utp_iteration.thy                                                    *)
+(* Author: Simon Foster and Frank Zeyda, University of York (UK)              *)
+(******************************************************************************)
+
+header {* Constructs for Iteration *}
+
+theory utp_iteration
+imports 
+  utp_recursion
+  "../laws/utp_refine_laws"
+begin
+
+text {* Relational Iteration (Kleene Star) *}
+
+lemma OneP_closure [closure]:
+  "1 \<in> WF_RELATION"
+  by (simp add:one_WF_PREDICATE_def closure)
+
+lemma TimesP_closure [closure]:
+  "\<lbrakk> P \<in> WF_RELATION; Q \<in> WF_RELATION \<rbrakk> \<Longrightarrow> P\<cdot>Q \<in> WF_RELATION"
+  by (simp add:times_WF_PREDICATE_def closure)
+
+lemma PowerP_closure [closure]:
+  fixes P :: "'a WF_PREDICATE"
+  assumes "P \<in> WF_RELATION"
+  shows "P^n \<in> WF_RELATION"
+  by (induct n, simp_all add:closure assms)
+  
+lemma EvalRR_power [evalrr]:
+  "\<lbrakk>P^n\<rbrakk>\<R> = \<lbrakk>P\<rbrakk>\<R> ^^ n"
+  apply (induct n)
+  apply (simp add:one_WF_PREDICATE_def evalrr)
+  apply (simp add:times_WF_PREDICATE_def evalrr relpow_commute)
+done
+
+lemma EvalRX_power [evalrx]:
+  "P \<in> WF_RELATION \<Longrightarrow> \<lbrakk>P^n\<rbrakk>RX = \<lbrakk>P\<rbrakk>RX ^^ n"
+  apply (induct n)
+  apply (simp add:one_WF_PREDICATE_def evalrx)
+  apply (simp add:times_WF_PREDICATE_def evalrx closure relpow_commute)
+done
+
+lemma UNREST_PowerP [unrest]: "UNREST NON_REL_VAR p \<Longrightarrow> UNREST NON_REL_VAR (p ^ n)"
+  apply (induct n)
+  apply (simp add:unrest one_WF_PREDICATE_def)
+  apply (simp add:times_WF_PREDICATE_def)
+  apply (force intro:unrest)
+done
+
+instantiation WF_PREDICATE :: (VALUE) star_op
+begin
+
+definition star_WF_PREDICATE :: "'a WF_PREDICATE \<Rightarrow> 'a WF_PREDICATE" where
+"star_WF_PREDICATE p \<equiv> (\<Sqinter> { p ^ n | n. n \<in> UNIV})"
+
+instance ..
+
+end
+
+syntax
+  "_upred_star"     :: "upred \<Rightarrow> upred" ("_\<^sup>\<star>" [101] 100)
+
+translations
+  "_upred_star p"   == "p\<^sup>\<star>"
+
+lemma StarP_closure [closure]:
+  "P \<in> WF_RELATION \<Longrightarrow> P\<^sup>\<star> \<in> WF_RELATION"
+  by (auto intro:closure simp add:star_WF_PREDICATE_def)
+
+lemma EvalRR_StarP: "\<lbrakk>P\<^sup>\<star>\<rbrakk>\<R> = \<lbrakk>P\<rbrakk>\<R>\<^sup>*"
+  apply (auto simp add: rtrancl_is_UN_relpow star_WF_PREDICATE_def evalrr)
+  apply (metis EvalRR_power)
+done
+
+lemma EvalRX_StarP [evalrx]: 
+  "P \<in> WF_RELATION \<Longrightarrow> \<lbrakk>P\<^sup>\<star>\<rbrakk>RX = \<lbrakk>P\<rbrakk>RX\<^sup>*"
+  apply (auto simp add: rtrancl_is_UN_relpow star_WF_PREDICATE_def evalrx closure)
+  apply (metis EvalRX_power)
+done
+
+lemma EvalRR_StarP_Union: "\<lbrakk>P\<^sup>\<star>\<rbrakk>\<R> = (\<Union>n. (\<lbrakk>P\<rbrakk>\<R> ^^ n))"
+  apply (auto simp add: rtrancl_is_UN_relpow star_WF_PREDICATE_def evalrr)
+  apply (metis EvalRR_power)
+done
+
+lemma EvalRX_StarP_Union: 
+  "P \<in> WF_RELATION \<Longrightarrow> \<lbrakk>P\<^sup>\<star>\<rbrakk>RX = (\<Union>n. (\<lbrakk>P\<rbrakk>RX ^^ n))"
+  apply (auto simp add: rtrancl_is_UN_relpow star_WF_PREDICATE_def evalrx closure)
+  apply (metis EvalRX_power)
+done
+
+lemma UNREST_StarP [unrest]: "UNREST NON_REL_VAR p \<Longrightarrow> UNREST NON_REL_VAR (p\<^sup>\<star>)"
+  by (auto intro:unrest simp add:star_WF_PREDICATE_def)
+
+instantiation WF_PREDICATE :: (VALUE) dioid
+begin
+
+instance
+  apply (intro_classes)
+  apply (simp_all add:plus_WF_PREDICATE_def times_WF_PREDICATE_def 
+                      zero_WF_PREDICATE_def one_WF_PREDICATE_def
+                      less_WF_PREDICATE_def)
+  apply (utp_pred_auto_tac)+
+done
+end
+
+instantiation WF_PREDICATE :: (VALUE) kleene_algebra
+begin
+
+instance proof
+
+  fix x :: "'a WF_PREDICATE"
+  show "x\<^sup>\<star> \<sqsubseteq> 1 + x \<cdot> x\<^sup>\<star>"
+    by (auto simp add: evalrr EvalRR_StarP)
+
+next
+
+  fix x y z :: "'a WF_PREDICATE"
+  show "y \<sqsubseteq> z + x \<cdot> y \<longrightarrow> y \<sqsubseteq> x\<^sup>\<star> \<cdot> z"
+    apply (simp add: evalrr EvalRR_StarP)
+    apply (metis rel_dioid.add_lub rel_kleene_algebra.star_inductl)
+  done
+
+next
+
+  fix x y z :: "'a WF_PREDICATE"
+  show "y \<sqsubseteq> z + y \<cdot> x \<longrightarrow> y \<sqsubseteq> z \<cdot> x\<^sup>\<star>"
+    apply (simp add: evalrr EvalRR_StarP)
+    apply (metis Un_least rel_kleene_algebra.star_inductr)
+  done
+
+qed (simp_all add: evalrr)
+end
+
+lemma StarP_mono: "mono (\<lambda> x. (II \<or>\<^sub>p (p ; x)))"
+  apply (rule)
+  apply (utp_rel_auto_tac)
+done
+lemma StarP_WFP1: "(\<mu> X \<bullet> II \<or>\<^sub>p (P ; X)) \<sqsubseteq> P\<^sup>\<star>"
+  apply (auto simp add:evalrr EvalRR_StarP gfp_def)
+  apply (metis EvalRR_StarP rel_kleene_algebra.star_unfoldl_eq subset_refl)
+done
+
+lemma StarP_WFP2: "P\<^sup>\<star> \<sqsubseteq> (\<mu> X \<bullet> II \<or>\<^sub>p (P ; X))"
+  apply (auto simp add:evalrr EvalRR_StarP_Union gfp_def)
+oops
+
+definition 
+  IterP :: " 'a WF_PREDICATE 
+           \<Rightarrow> 'a WF_PREDICATE 
+           \<Rightarrow> 'a WF_PREDICATE" ("while _ do _ od") where
+"IterP b P \<equiv> (P \<lhd> b \<rhd> II)\<^sup>\<star>"
+
+syntax
+  "_upred_while"    :: "upred \<Rightarrow> upred \<Rightarrow> upred" ("while _ do _ od")
+
+translations
+  "_upred_while b p"   == "CONST IterP b p"
+
+declare EvalRR_StarP [evalrr]
+declare IterP_def [eval, evalr, evalrr, evalrx]
+
+lemma IterP_closure [closure]:
+  "\<lbrakk> b \<in> WF_RELATION; P \<in> WF_RELATION \<rbrakk> \<Longrightarrow>
+     while b do P od \<in> WF_RELATION"
+  by (simp add:IterP_def closure)
+
+theorem IterP_refine [refine]:
+  "while b do P od \<sqsubseteq> (P \<lhd> b \<rhd> II) ; (while b do P od)"
+  by (metis IterP_def star_1l times_WF_PREDICATE_def)
+  
+theorem IterP_false: "while false do P od = II"
+  by (simp add:evalrr)
+theorem IterP_true: "while true do P od = P\<^sup>\<star>"
+  by (simp add:evalrr)
+
+theorem IterP_cond_true_refine [refine]:
+  assumes "b \<in> WF_CONDITION" "P \<in> WF_RELATION"
+  shows "`(while b do P od) \<and> b` \<sqsubseteq> `(P \<and> b) ; while b do P od`"
+proof -
+
+  have "`while b do P od \<and> b` \<sqsubseteq> `((P \<lhd> b \<rhd> II) ; (while b do P od)) \<and> b`" (is "?l \<sqsubseteq> ?r")
+    by (metis AndP_mono_refine IterP_refine order_refl)
+
+  also have "?r = `b \<and> ((P \<lhd> b \<rhd> II) ; while b do P od)`"
+    by (metis AndP_comm)
+
+  also have "... = `((P \<and> b) ; while b do P od)`"
+    by (metis AndP_comm CondR_rel_closure CondR_true_cond IterP_closure SemiR_AndP_left_precond SkipR_closure WF_CONDITION_WF_RELATION assms)
+
+  finally show ?thesis ..
+qed
+
+theorem IterP_cond_false_refine [refine]:
+  assumes "b \<in> WF_CONDITION" "P \<in> WF_RELATION"
+  shows "`(while b do P od) \<and> \<not>b` \<sqsubseteq> `II \<and> \<not>b`"
+  using assms
+  apply (simp add:IterP_def)
+  apply (frule SemiR_TrueP_precond)
+  apply (utp_xrel_auto_tac)
+done
+
+end
